compacting the tree

examples/data_structures/BinomialQueue.fst
@@ -30,7 +30,90 @@ let rec is_ith_tail (i:pos) (l:list tree)
   | hd::tl ->
     (Leaf? hd \/ is_pow2heap i hd) /\ is_ith_tail (i + 1) tl
 
-type priq = l:list tree{is_ith_tail 1 l}
+let rec all_leaf (l:list tree{Cons? l}) : bool =
+  match l with
+  | [Leaf] -> true
+  | Leaf::tl -> all_leaf tl
+  | _ -> false
+
+let rec mk_compact (l:list tree) : list tree =
+  match l with
+  | [] -> []
+  | _ ->
+    if all_leaf l then []
+    else let hd::tl = l in
+         hd::(mk_compact tl)
+
+let mk_compact_length (l:list tree{Cons? l})
+  : Lemma (requires not (all_leaf l))
+          (ensures L.length (mk_compact l) > 0)
+  = ()
+
+let last_cons (#a:Type) (x:a) (l:list a)
+  : Lemma
+      (requires Cons? l)
+      (ensures L.last (x::l) == L.last l)
+      [SMTPat (L.last (x::l))]
+  = admit ()
+    
+let is_compact (l:list tree) = l == [] \/ Internal? (L.last l)
+
+let rec mk_compact_correctness (l:list tree)
+  : Lemma (is_compact (mk_compact l))
+          [SMTPat (is_compact (mk_compact l))] =
+
+  match l with
+  | [] -> ()
+  | _ ->
+    if all_leaf l then ()
+    else mk_compact_correctness (L.tl l)
+
+let rec mk_compact_preserves_ith_tail (i:pos) (l:list tree)
+  : Lemma
+      (requires is_ith_tail i l)
+      (ensures is_ith_tail i (mk_compact l))
+      (decreases l)
+      [SMTPat (is_ith_tail i (mk_compact l))] =
+  match l with
+  | [] -> ()
+  | _ ->
+    if all_leaf l then ()
+    else mk_compact_preserves_ith_tail (i + 1) (L.tl l)
+
+let rec keys_of_tree (t:tree) : list key_t =
+  match t with
+  | Leaf -> []
+  | Internal left k right ->
+    L.append (keys_of_tree left)
+             (L.append [k] (keys_of_tree right))
+
+let rec keys (q:list tree) : list key_t =
+  match q with
+  | [] -> []
+  | hd::tl -> L.append (keys_of_tree hd) (keys tl)
+
+let rec all_leaf_keys (l:list tree{Cons? l})
+  : Lemma
+      (requires Cons? l /\ all_leaf l)
+      (ensures keys l == []) =
+  match l with
+  | [Leaf] -> ()
+  | Leaf::tl -> all_leaf_keys tl
+
+let rec compact_preserves_keys (q:list tree)
+  : Lemma (keys q == keys (mk_compact q))
+          [SMTPat (keys (mk_compact q))] =
+
+  match q with
+  | [] -> ()
+  | _ ->
+    if all_leaf q
+    then all_leaf_keys q
+    else compact_preserves_keys (L.tl q)
+    
+let is_priq (l:list tree) = is_ith_tail 1 l /\ is_compact l
+
+type priq = l:list tree{is_priq l}
 
 let empty : priq = []
 
@@ -105,6 +188,7 @@ let rec unzip (depth:nat) (upper_bound:key_t) (t:tree)
     let q = unzip (depth - 1) upper_bound right in
     priq_append q (Internal left k Leaf);
     L.append_length q [Internal left k Leaf];
+    assume (is_priq (L.append q [Internal left k Leaf]));
     L.append q [Internal left k Leaf]
 
 let heap_delete_max (depth:pos) (t:tree)
@@ -148,10 +232,12 @@ let delete_max (q:priq) : option (key_t & priq) =
   | Some m ->
     let q, new_q = delete_max_aux m 1 q in
     let r = join 1 q new_q Leaf in
-    Some (m, r)
+    mk_compact_correctness r;
+    Some (m, mk_compact r)
 
 let insert (x:key_t) (q:priq) : priq =
-  carry 1 q (Internal Leaf x Leaf)
+  let l = carry 1 q (Internal Leaf x Leaf) in
+  mk_compact l
 
 let count_elt (x:key_t) (hd:key_t) : nat =
   if x = hd then 1 else 0
@@ -179,23 +265,11 @@ let permutation_append (l1 l2 l3 l4:list key_t)
       (ensures permutation (l1@l2) (l3@l4)) =
   ()
 
-let rec keys_of_tree (t:tree) : list key_t =
-  match t with
-  | Leaf -> []
-  | Internal left k right ->
-    L.append (keys_of_tree left)
-             (L.append [k] (keys_of_tree right))
-
-let rec keys_of_priq (q:list tree) : list key_t =
-  match q with
-  | [] -> []
-  | hd::tl -> L.append (keys_of_tree hd) (keys_of_priq tl)
-
 let represents_t (t:tree) (l:list key_t) : prop =
   permutation (keys_of_tree t) l
 
 let represents (q:list tree) (l:list key_t) : prop =
-  permutation (keys_of_priq q) l
+  permutation (keys q) l
 
 let permutation_represents (l1 l2:list key_t) (q:priq)
   : Lemma
@@ -213,17 +287,17 @@ let represents_permutation (l1 l2:list key_t) (q:priq)
       (ensures permutation l1 l2)
   = ()
 
-let empty_relate (l:list key_t)
-  : Lemma (requires [] `represents` l)
-          (ensures l == [])
-          [SMTPat ([] `represents` l)] =
-  admit ()
+// let empty_relate (l:list key_t)
+//   : Lemma (requires [] `represents` l)
+//           (ensures l == [])
+//           [SMTPat ([] `represents` l)] =
+//   admit ()
 
-let leaf_relate (l:list key_t)
-  : Lemma (requires Leaf `represents_t` l)
-          (ensures l == [])
-          [SMTPat (Leaf `represents_t` l)] =
-  admit ()
+// let leaf_relate (l:list key_t)
+//   : Lemma (requires Leaf `represents_t` l)
+//           (ensures l == [])
+//           [SMTPat (Leaf `represents_t` l)] =
+//   admit ()
 
 let smash_represents (depth:nat) (t1 t2:tree) (l1 l2:list key_t)
   : Lemma
@@ -263,10 +337,10 @@ let rec carry_represents (depth:nat) (q:list tree) (t:tree) (lq lt:list key_t)
   | hd::tl ->
     smash_represents depth hd t (keys_of_tree hd) (keys_of_tree t);
     carry_represents (depth + 1) tl (smash depth hd t)
-      (keys_of_priq tl)
+      (keys tl)
       (L.append (keys_of_tree hd) (keys_of_tree t));
 
-    L.append_assoc (keys_of_priq tl) (keys_of_tree hd) (keys_of_tree t)
+    L.append_assoc (keys tl) (keys_of_tree hd) (keys_of_tree t)
 
 let permutation_cons_snoc (x:key_t) (l:list key_t)
   : Lemma (permutation (x::l) (l @ [x])) = admit ()
@@ -279,7 +353,7 @@ let insert_represents (x:key_t) (q:priq) (l:list key_t)
   carry_represents 1 q (Internal Leaf x Leaf) l [x];
   permutation_cons_snoc x l
 
-#push-options "--z3rlimit 40 --fuel 1 --ifuel 1"
+#push-options "--z3rlimit 100 --fuel 1 --ifuel 1"
 let rec join_represents (depth:nat) (p q:list tree) (c:tree)
   (lp lq lc:list key_t)
   : Lemma
@@ -303,132 +377,134 @@ let rec join_represents (depth:nat) (p q:list tree) (c:tree)
 
   | Leaf::tl_p, Leaf::tl_q, _ ->
     join_represents (depth + 1) tl_p tl_q Leaf
-      (keys_of_priq tl_p) (keys_of_priq tl_q) [];
-    L.append_l_nil (keys_of_priq tl_q);
+      (keys tl_p) (keys tl_q) [];
+    L.append_l_nil (keys tl_q);
     assert (permutation
               (keys_of_tree c @
-               (keys_of_priq tl_p @ keys_of_priq tl_q))
-              ((keys_of_priq tl_p @ keys_of_priq tl_q) @
+               (keys tl_p @ keys tl_q))
+              ((keys tl_p @ keys tl_q) @
                keys_of_tree c));
-    L.append_assoc (keys_of_priq tl_p)
-                   (keys_of_priq tl_q)
+    L.append_assoc (keys tl_p)
+                   (keys tl_q)
                    (keys_of_tree c)
 
   | hd_p::tl_p, Leaf::tl_q, Leaf ->
     join_represents (depth + 1) tl_p tl_q Leaf
-      (keys_of_priq tl_p) (keys_of_priq tl_q) [];
+      (keys tl_p) (keys tl_q) [];
 
-    L.append_assoc (keys_of_tree hd_p) (keys_of_priq tl_p) 
-                   (keys_of_priq tl_q @ []);
+    L.append_assoc (keys_of_tree hd_p) (keys tl_p) 
+                   (keys tl_q @ []);
     
-    permutation_append (keys_of_priq q)
+    permutation_append (keys q)
                        []
                        lq
                        lc;
-    permutation_append (keys_of_priq p)
-                       ((keys_of_priq q) @ [])
+    permutation_append (keys p)
+                       ((keys q) @ [])
                        lp
                        (lq @ lc)
   | Leaf::tl_p, hd_q::tl_q, Leaf ->
     join_represents (depth + 1) tl_p tl_q Leaf
-      (keys_of_priq tl_p) (keys_of_priq tl_q) [];
-    L.append_l_nil (keys_of_priq tl_q);
+      (keys tl_p) (keys tl_q) [];
+    L.append_l_nil (keys tl_q);
 
     assert (r `represents`
             (keys_of_tree hd_q @
-             (keys_of_priq tl_p @ keys_of_priq tl_q)));
+             (keys tl_p @ keys tl_q)));
 
     assume (permutation
               (keys_of_tree hd_q @
-               (keys_of_priq tl_p @ keys_of_priq tl_q))
-              (keys_of_priq tl_p @ (keys_of_tree hd_q @ keys_of_priq tl_q)));
+               (keys tl_p @ keys tl_q))
+              (keys tl_p @ (keys_of_tree hd_q @ keys tl_q)));
 
-    permutation_append (keys_of_priq q)
+    permutation_append (keys q)
                        []
                        lq
                        lc;
-    permutation_append (keys_of_priq p)
-                       ((keys_of_priq q) @ [])
+    permutation_append (keys p)
+                       ((keys q) @ [])
                        lp
                        (lq @ lc)
   | Leaf::tl_p, hd_q::tl_q, _ ->
     smash_represents depth hd_q c (keys_of_tree hd_q) (keys_of_tree c);
     join_represents (depth + 1) tl_p tl_q (smash depth hd_q c)
-      (keys_of_priq tl_p) (keys_of_priq tl_q)
+      (keys tl_p) (keys tl_q)
       (L.append (keys_of_tree hd_q) (keys_of_tree c));
 
     assert (r `represents`
-            (keys_of_priq tl_p @
-             (keys_of_priq tl_q @ (keys_of_tree hd_q @ keys_of_tree c))));
+            (keys tl_p @
+             (keys tl_q @ (keys_of_tree hd_q @ keys_of_tree c))));
 
     assume (permutation
-              (keys_of_priq tl_p @
-               (keys_of_priq tl_q @ (keys_of_tree hd_q @ keys_of_tree c)))
-              (keys_of_priq tl_p @ ((keys_of_tree hd_q @ keys_of_priq tl_q) @ keys_of_tree c)));
+              (keys tl_p @
+               (keys tl_q @ (keys_of_tree hd_q @ keys_of_tree c)))
+              (keys tl_p @ ((keys_of_tree hd_q @ keys tl_q) @ keys_of_tree c)));
 
-    permutation_append (keys_of_priq q)
+    permutation_append (keys q)
                        (keys_of_tree c)
                        lq
                        lc;
-    permutation_append (keys_of_priq p)
-                       ((keys_of_priq q) @ keys_of_tree c)
+    permutation_append (keys p)
+                       ((keys q) @ keys_of_tree c)
                        lp
                        (lq @ lc)
 
   | hd_p::tl_p, Leaf::tl_q, _ ->
     smash_represents depth hd_p c (keys_of_tree hd_p) (keys_of_tree c);
     join_represents (depth + 1) tl_p tl_q (smash depth hd_p c)
-      (keys_of_priq tl_p) (keys_of_priq tl_q)
+      (keys tl_p) (keys tl_q)
       (L.append (keys_of_tree hd_p) (keys_of_tree c));
 
     assert (r `represents`
-            (keys_of_priq tl_p @
-             (keys_of_priq tl_q @ (keys_of_tree hd_p @ keys_of_tree c))));
+            (keys tl_p @
+             (keys tl_q @ (keys_of_tree hd_p @ keys_of_tree c))));
 
     assume (permutation
-              (keys_of_priq tl_p @
-               (keys_of_priq tl_q @ (keys_of_tree hd_p @ keys_of_tree c)))
-              ((keys_of_tree hd_p @ keys_of_priq tl_p) @
-               (keys_of_priq tl_q @ keys_of_tree c)));
+              (keys tl_p @
+               (keys tl_q @ (keys_of_tree hd_p @ keys_of_tree c)))
+              ((keys_of_tree hd_p @ keys tl_p) @
+               (keys tl_q @ keys_of_tree c)));
 
-    permutation_append (keys_of_priq q)
+    permutation_append (keys q)
                        (keys_of_tree c)
                        lq
                        lc;
-    permutation_append (keys_of_priq p)
-                       ((keys_of_priq q) @ keys_of_tree c)
+    permutation_append (keys p)
+                       ((keys q) @ keys_of_tree c)
                        lp
                        (lq @ lc)
 
   | hd_p::tl_p, hd_q::tl_q, c ->
     smash_represents depth hd_p hd_q (keys_of_tree hd_p) (keys_of_tree hd_q);
     join_represents (depth + 1) tl_p tl_q (smash depth hd_p hd_q)
-      (keys_of_priq tl_p) (keys_of_priq tl_q)
+      (keys tl_p) (keys tl_q)
       (L.append (keys_of_tree hd_p) (keys_of_tree hd_q));
     
     assert (r `represents`
             (keys_of_tree c @
-             (keys_of_priq tl_p @
-              (keys_of_priq tl_q @ (keys_of_tree hd_p @ keys_of_tree hd_q)))));
+             (keys tl_p @
+              (keys tl_q @ (keys_of_tree hd_p @ keys_of_tree hd_q)))));
 
     assume (permutation
               (keys_of_tree c @
-               (keys_of_priq tl_p @
-                (keys_of_priq tl_q @ (keys_of_tree hd_p @ keys_of_tree hd_q))))
-              ((keys_of_tree hd_p @ keys_of_priq tl_p) @
-               ((keys_of_tree hd_q @ keys_of_priq tl_q) @
+               (keys tl_p @
+                (keys tl_q @ (keys_of_tree hd_p @ keys_of_tree hd_q))))
+              ((keys_of_tree hd_p @ keys tl_p) @
+               ((keys_of_tree hd_q @ keys tl_q) @
                 (keys_of_tree c))));
     admit ();
-    permutation_append (keys_of_priq q)
+    permutation_append (keys q)
                        (keys_of_tree c)
                        lq
                        lc;
-    permutation_append (keys_of_priq p)
-                       ((keys_of_priq q) @ keys_of_tree c)
+    permutation_append (keys p)
+                       ((keys q) @ keys_of_tree c)
                        lp
                        (lq @ lc)
 
-let merge (p q:priq) : priq = join 1 p q Leaf
+let merge (p q:priq) : priq =
+  let l = join 1 p q Leaf in
+  mk_compact l
 
 let merge_representation (p q:priq) (lp lq:list key_t)
   : Lemma
@@ -436,4 +512,3 @@ let merge_representation (p q:priq) (lp lq:list key_t)
       (ensures merge p q `represents` (lp @ lq)) =
 
   join_represents 1 p q Leaf lp lq []
-
